fiat2/src/fiat2/ParamPipelineEx.v
@@ -1,0 +1,389 @@
+Require Import fiat2.Language fiat2.Interpret fiat2.Value fiat2.TypeSystem fiat2.TypeSound fiat2.IndexInterface
+  fiat2.CollectionTransf fiat2.DictIndexImpl fiat2.SumAgg fiat2.MinAgg fiat2.BitmapIndex fiat2.TransfUtils fiat2.RelTransf fiat2.IndexTransf fiat2.TransfSound fiat2.Utils fiat2.Substitute.
+Require Import coqutil.Map.Interface coqutil.Map.SortedListString coqutil.Word.Interface coqutil.Datatypes.Result.
+Require Import List String ZArith.
+Import ListNotations.
+
+Require Import fiat2.Notations.
+Open Scope fiat2_scope.
+
+Section WithConcreteMaps.
+  Context {width: Z} {word: word.word width} {word_ok: word.ok word}.
+  Notation value := (value (width:=width)).
+
+  Local Open Scope string.
+
+  Instance ctenv : map.map string type := SortedListString.map _.
+  Instance ctenv_ok : map.ok ctenv := SortedListString.ok _.
+
+  Instance clocals : map.map string value := SortedListString.map _.
+  Instance clocals_ok : map.ok clocals := SortedListString.ok _.
+
+  Section CommonPipelineParts.
+    Context (sum_agg_attr : string).
+
+    Definition sum_agg_wf := (SumAgg.idx_wf (locals:=clocals) "hole" sum_agg_attr "x").
+    Instance csum_agg : IndexInterface.index := (sum_agg "hole" sum_agg_attr "x").
+    Instance csum_agg_ok : IndexInterface.ok csum_agg sum_agg_wf.
+    apply sum_agg_ok.
+    Qed.
+
+    Definition sum_agg_lookup_transf := fun tbl => fold_command_with_globals [tbl] (sum_to_agg_lookup_head sum_agg_attr "id_tag" "aux_tag" "sum_agg_tag" tbl).
+    Definition cons_to_add_transf := fun tbl => fold_command_with_globals [tbl] (cons_to_add_head).
+
+    Context (min_agg_attr : string).
+
+    Definition min_agg_wf := (MinAgg.idx_wf (locals:=clocals) "hole" min_agg_attr "x").
+    Instance cmin_agg : IndexInterface.index := (min_agg "hole" min_agg_attr "x").
+    Instance cmin_agg_ok : IndexInterface.ok cmin_agg min_agg_wf.
+    apply min_agg_ok.
+    Qed.
+
+    Definition min_agg_lookup_transf := fun tbl => fold_command_with_globals [tbl] (min_to_agg_lookup_head min_agg_attr "id_tag" "aux_tag" "min_agg_tag" tbl).
+    Definition cons_to_min_transf := fun tbl => fold_command_with_globals [tbl] (cons_to_min_head "y").
+
+    Context (dict_idx_attr : string).
+
+    Definition dict_idx_wf := (DictIndexImpl.idx_wf (width:=width) "hole" dict_idx_attr "tup" "acc" "x").
+    Instance cdict_idx : IndexInterface.index := (dict_idx "hole" dict_idx_attr "tup" "acc" "x").
+    Instance cdict_idx_ok : IndexInterface.ok cdict_idx dict_idx_wf.
+    apply dict_idx_ok. auto with transf_hints.
+    Qed.
+
+    Definition dict_lookup_transf := fun tbl => fold_command_with_globals [tbl] (eq_filter_to_lookup_head dict_idx_attr "id_tag" "aux_tag" "dict_idx_tag" "b" tbl).
+    Definition cons_to_insert_transf := fun tbl => fold_command_with_globals [tbl] (cons_to_insert_head dict_idx_attr "tup" "acc" "x" "y").
+    Definition use_dict_idx_transf := fun tbl => fold_command_with_globals [tbl] (use_idx_head dict_idx_attr "id_tag" "aux_tag" "dict_idx_tag" tbl).
+
+    Definition pk_idx_wf := (BitmapIndex.pk_idx_wf (width:=width) "hole" "tup" "acc").
+    Instance cpk_idx : IndexInterface.index := (pk_idx "hole" "tup" "acc").
+    Instance cpk_idx_ok : IndexInterface.ok cpk_idx pk_idx_wf.
+    apply pk_idx_ok. auto with transf_hints.
+    Qed.
+
+    Context (bitmap_attr : string).
+    Context (bitmap_str : string).
+    Definition bitmap_wf := (bitmap_wf (width:=width) bitmap_attr bitmap_str "hole" "tup").
+    Instance bitmap : IndexInterface.index := (bitmap bitmap_attr bitmap_str "hole" "tup").
+    Instance bitmap_ok : IndexInterface.ok bitmap bitmap_wf.
+    apply bitmap_ok.
+    Qed.
+
+    Definition cons_to_pk_idx_update_transf := fun tbl => fold_command_with_globals [tbl] (cons_to_pk_idx_update_head "y").
+    Definition use_pk_idx_transf := fun tbl => fold_command_with_globals [tbl] (use_pk_idx_head "id_tag" "aux_tag" "pk_idx_tag" tbl).
+    Definition cons_to_bitmap_update_transf := fun tbl => fold_command_with_globals [tbl] cons_to_bitmap_update_head.
+    Definition use_bitmap_transf := fun tbl => fold_command_with_globals [tbl] (use_bitmap_head bitmap_attr bitmap_str "id_tag" "aux_tag" "bm_tag" tbl).
+    Definition filter_to_bitmap_lookup_transf :=
+      fun tbl => fold_command_with_globals [tbl]
+                   (filter_to_bitmap_lookup_head bitmap_attr bitmap_str "id_tag" "aux_tag" "pk_idx_tag" "bm_tag" "x" "b" "acc" tbl).
+  End CommonPipelineParts.
+
+  Section ParameterizedPipeline.
+    Context (sum_agg_attr : option string).
+    Context (min_agg_attr : option string).
+    Context (dict_idx_attr : option string).
+    Context (bitmap_params : option (string * string)).
+
+    Definition to_proj_transf := fold_command id to_proj_head.
+    Definition to_filter_transf := fold_command id to_filter_head.
+    Definition to_join_transf := fold_command id to_join_head.
+    Definition annotate_collection_transf := fold_command id annotate_collection.
+    Definition push_down_collection_transf := fold_command id push_down_collection.
+    Definition filter_pushdown_transf := fold_command id filter_pushdown_head.
+
+    Notation idxs :=
+      (match sum_agg_attr with
+       | None => []
+       | Some sum_agg_attr =>
+           [("sum_agg_tag", csum_agg sum_agg_attr, sum_agg_wf sum_agg_attr)]
+       end ++
+         match min_agg_attr with
+         | None => []
+         | Some min_agg_attr =>
+             [("min_agg_tag", cmin_agg min_agg_attr, min_agg_wf min_agg_attr)]
+         end ++
+         match dict_idx_attr with
+         | None => []
+         | Some dict_idx_attr =>
+             [("dict_idx_tag", cdict_idx dict_idx_attr, dict_idx_wf dict_idx_attr)]
+         end ++
+         match bitmap_params with
+         | None => []
+         | Some (bitmap_attr, bitmap_str) =>
+             [("pk_idx_tag", cpk_idx, pk_idx_wf);
+              ("bm_tag", bitmap bitmap_attr bitmap_str, bitmap_wf bitmap_attr bitmap_str)]
+         end)%list.
+
+    Instance ccompo_idx : IndexInterface.index := compo_idx idxs "hole" (word:=word).
+    Instance ccompo_idx_ok : IndexInterface.ok ccompo_idx (compo_idx_wf idxs).
+    apply compo_idx_ok;
+      repeat case_match;
+      repeat constructor; intros; auto with transf_hints;
+      cbn; rewrite <- eqb_eq; intuition idtac; discriminate.
+    Qed.
+
+    Definition ex_transf (Gstore Genv : ctenv) :=
+      Basics.compose
+        (apply_idx_related_transfs (idx:=ccompo_idx) "id_tag" "aux_tag"
+           (fun tbl =>
+              (Basics.compose
+                 (match bitmap_params with
+                  | Some (bitmap_attr, bitmap_str) =>
+                      Basics.compose (filter_to_bitmap_lookup_transf bitmap_attr bitmap_str tbl)
+                        (Basics.compose (use_bitmap_transf bitmap_attr bitmap_str tbl)
+                           (Basics.compose (repeat_transf (cons_to_bitmap_update_transf tbl) 10000)
+                              (Basics.compose (use_pk_idx_transf tbl) (repeat_transf (cons_to_pk_idx_update_transf tbl) 10000))))
+                  | None => id
+                  end)
+                 (Basics.compose
+                    match dict_idx_attr with
+                    | Some dict_idx_attr =>
+                        Basics.compose (dict_lookup_transf dict_idx_attr tbl)
+                          (Basics.compose (use_dict_idx_transf dict_idx_attr tbl)
+                             (repeat_transf (cons_to_insert_transf dict_idx_attr tbl) 10000))
+                    | None => id
+                    end
+                    (Basics.compose
+                       match min_agg_attr with
+                       | Some min_agg_attr =>
+                           Basics.compose (min_agg_lookup_transf min_agg_attr tbl)
+                             (repeat_transf (cons_to_min_transf tbl) 10000)
+                       | None => id
+                       end
+                       match sum_agg_attr with
+                       | Some sum_agg_attr =>
+                           Basics.compose (sum_agg_lookup_transf sum_agg_attr tbl)
+                             (repeat_transf (cons_to_add_transf tbl) 10000)
+                       | None => id
+                       end)))) Gstore Genv)
+           (Basics.compose push_down_collection_transf
+              (Basics.compose annotate_collection_transf
+                 (Basics.compose filter_pushdown_transf
+                    (Basics.compose to_filter_transf
+                       (Basics.compose to_proj_transf to_join_transf))))).
+
+    Lemma id_aug_transf_sound : forall is_tbl_ty aux_ty (aux_wf : value -> Prop),
+        aug_transf_sound is_tbl_ty aux_ty aux_wf (fun _ => id).
+    Proof.
+      unfold aug_transf_sound; cbn; auto.
+    Qed.
+
+    Lemma ex_transf_sound : transf_sound (locals:=clocals) ex_transf.
+    Proof.
+      unfold ex_transf.
+      repeat case_match;
+        repeat (repeat apply_transf_sound_lemmas; eauto 10 with transf_hints).
+      all:
+        try simple eapply id_aug_transf_sound;
+        try simple eapply filter_to_bitmap_lookup_head_sound2;
+        try simple eapply use_bitmap_head_sound;
+        try simple eapply use_pk_idx_head_sound2;
+        try simple eapply use_idx_head_sound2;
+        try simple eapply min_to_agg_lookup_head_sound;
+        try simple eapply sum_to_agg_lookup_head_sound;
+        try simple eapply eq_filter_to_lookup_head_sound2;
+        eauto with transf_hints;
+        try (unfold aux_ty_for_idx, aux_ty; cbn;
+             repeat rewrite_l_to_r;
+             eauto with transf_hints);
+        try (unfold compo_is_tbl_ty;
+             unfold IndexInterface.is_tbl_ty; cbn; intros;
+             rewrite !Bool.andb_true_iff in *; intuition idtac);
+        try (intros; unfold aux_wf, aux_wf_for_idx, compo_idx_wf in *;
+             repeat destruct_match_hyp; intuition idtac; cbn in *;
+             repeat invert_Forall;
+             case_match; intuition idtac;
+             eauto with transf_hints);
+        try use_is_NoDup.
+    Qed.
+  End ParameterizedPipeline.
+
+  Section ExampleFilterPushdown.
+    Definition row_ty1 := TRecord (record_sort [("A", TInt); ("B", TString)]).
+    Definition row_ty2 := TRecord (record_sort [("B", TString); ("C", TInt)]).
+
+    Definition ex_pushdown :=
+      <[ "r1" <- "tbl1";
+         "r2" <- "tbl2";
+         check("r1"["A"] == 0 && "r1"["B"] == "r2"["B"]);
+         ret {"B": "r1"["B"], "C": "r2"["C"]} ]>.
+
+    Definition ex0 := CAssign "res" ex_pushdown.
+
+    Definition init_Gstore0 : ctenv := map.put map.empty "res" (TList (TRecord ([("B", TString); ("C", TInt)]))).
+    Definition init_Genv0 : ctenv := map.put (map.put map.empty "tbl1" (TList row_ty1)) "tbl2" (TList row_ty2).
+
+    Definition ex_transf_pushdown := ex_transf None None None None.
+    Definition ex0_transformed := ex_transf_pushdown init_Gstore0 init_Genv0 ex0.
+    (* Compute (typecheck init_Gstore0 init_Genv0 ex0). *)
+    (* Compute ex0_transformed. *)
+
+    Theorem ex0_transformed_sem : forall (store env : clocals),
+        locals_wf init_Gstore0 store ->
+        locals_wf init_Genv0 env ->
+        interp_command store env ex0_transformed = interp_command store env ex0.
+    Proof.
+      apply transf_sound__preserve_sem; eauto using ex_transf_sound with transf_hints.
+    Qed.
+  End ExampleFilterPushdown.
+
+
+  Section Example1.
+    Definition sum_agg_attr1 := "salary".
+    Definition dict_idx_attr1 := "department".
+    Definition bitmap_attr1 := "location".
+    Definition bitmap_str1 := "A".
+
+    Definition ex_transf1 := ex_transf (Some sum_agg_attr1) None (Some dict_idx_attr1) (Some (bitmap_attr1, bitmap_str1)).
+
+    Definition row_ty := TRecord (record_sort [("name", TString); ("department", TString); ("feedback", TString); ("salary", TInt); ("location", TString)]).
+    (* Two Arbitrary well_typed rows *)
+    Definition row1 := EVar "row1".
+    Definition row2 := EVar "row2".
+
+    Definition build_responses1 := <{ set "responses" := row1 :: row2 :: mut "responses" }>.
+    Definition filter_responses dpt : expr := ESort LikeList <[ "row" <- mut "responses" ;
+                                                                check("row"["department"] == << EAtom (AString dpt) >>);
+                                                                ret "row" ]>.
+    Definition filter_responses2 : expr := <[ "row" <- mut "responses" ;
+                                              check("row"["location"] == << EAtom (AString "A") >>);
+                                              ret "row" ]>.
+    Definition query1_1 := CForeach (filter_responses "CS") "r"
+                           <{ let "name" = "r"["name"] +++ << EAtom (AString ": ") >> in
+                              let "feedback" = "r"["feedback"] +++ << EAtom (AString "\n") >> in
+                              let "line" = "name" +++ "feedback" in
+                              set "all_feedback" := mut "all_feedback" +++ "line" }>.
+    Definition query1_2 := CAssign "sum" (EFold (<["row" <- mut "responses" ; ret "row"["salary"]]>) (EAtom (AInt 0)) "v" "acc" (EBinop OPlus (EVar "v") (EVar "acc"))).
+    Definition query1_3 := CForeach (filter_responses2) "r"
+                           <{ let "name" = "r"["name"] +++ << EAtom (AString ": ") >> in
+                              let "feedback" = "r"["feedback"] +++ << EAtom (AString "\n") >> in
+                              let "line" = "name" +++ "feedback" in
+                              set "all_feedback" := mut "all_feedback" +++ "line" }>.
+    Definition ex1' := CSeq build_responses1 (CSeq query1_1 (CSeq query1_2 query1_3)).
+    Definition ex1 := CLetMut (EAtom (ANil (Some (row_ty)))) "responses" ex1'.
+
+    Definition init_Gstore1 : ctenv := map.put (map.put map.empty "all_feedback" TString) "sum" TInt.
+    Definition init_Genv1 : ctenv := map.put (map.put map.empty "row1" row_ty) "row2" row_ty.
+
+    Definition ex1_transformed := ex_transf1 init_Gstore1 init_Genv1 ex1.
+    (* Compute typecheck init_Gstore1 init_Genv1 ex1. *)
+    (* Compute ex1_transformed. *)
+
+    Theorem ex1_transformed_sem : forall (store env : clocals),
+        locals_wf init_Gstore1 store ->
+        locals_wf init_Genv1 env ->
+        interp_command store env ex1_transformed = interp_command store env ex1.
+    Proof.
+      apply transf_sound__preserve_sem; eauto using ex_transf_sound with transf_hints.
+    Qed.
+  End Example1.
+
+  Section Example2.
+    Definition attr2 := "department-id".
+
+    Definition row_ty2_1 := TRecord (record_sort [("department-id", TInt); ("department-name", TString)]).
+    Definition row_ty2_2 := TRecord (record_sort [("name", TString); ("department-id", TInt); ("feedback", TString)]).
+
+    Definition join_tables : expr := ESort LikeList <[
+          "r1" <- mut "departments" ;
+          "r3" <- ("r2" <- mut "responses" ;
+                   check("r2"["department-id"] == "r1"["department-id"]);
+                   ret "r2") ;
+          ret {"name" : "r3" ["name"],
+                "department" : "r1" ["department-name"],
+                  "feedback" : "r3" ["feedback"]} ]>.
+
+    Definition ex2 := CLetMut (EVar "res_tbl") "responses"
+                        (CLetMut (EVar "dpt_tbl") "departments"
+                           (CForeach join_tables "r"
+                            <{ let "name" = "r"["name"] +++ << EAtom (AString " from ") >> in
+                               let "dep" = "r"["department"] +++ << EAtom (AString " wrote: ") >> in
+                               let "feedback" = "r"["feedback"] +++ << EAtom (AString "\n") >> in
+                               let "line" = "name" +++ "dep" +++ "feedback" in
+                               set "all_feedback" := mut "all_feedback" +++ "line" }>)).
+
+    Definition init_Gstore2 : ctenv := map.put map.empty "all_feedback" TString.
+    Definition init_Genv2 : ctenv := map.put (map.put map.empty "res_tbl" (TList row_ty2_2)) "dpt_tbl" (TList row_ty2_1).
+
+
+    Definition ex_transf2 := ex_transf None None (Some attr2) None.
+    Definition ex2_transformed := ex_transf2 init_Gstore2 init_Genv2 ex2.
+    (* Compute (typecheck init_Gstore1 init_Genv1 ex1). *)
+    (* Compute ex2_transformed. *)
+
+    Theorem ex2_transformed_sem : forall (store env : clocals),
+        locals_wf init_Gstore2 store ->
+        locals_wf init_Genv2 env ->
+        interp_command store env ex2_transformed = interp_command store env ex2.
+    Proof.
+      apply transf_sound__preserve_sem; eauto using ex_transf_sound with transf_hints.
+    Qed.
+  End Example2.
+
+  Section Example3.
+    Definition sum_agg_attr3 := "price".
+    Definition min_agg_attr3 := "price".
+    Definition dict_idx_attr3 := "color".
+    Definition bitmap_attr3 := "name".
+    Definition bitmap_str3 := "shirt_1".
+
+    Definition ex_transf3 := ex_transf (Some sum_agg_attr3) (Some min_agg_attr3) (Some dict_idx_attr3) (Some (bitmap_attr3, bitmap_str3)).
+
+    Definition outfits_row_ty := TRecord (record_sort [("outfit_name", TString); ("shirt_name", TString); ("shirt_color", TString); ("shirt_price", TInt); ("pants_name", TString); ("pants_color", TString); ("pants_price", TInt)]).
+
+    Definition shirts_row_ty := TRecord (record_sort [("name", TString); ("color", TString); ("price", TInt)]).
+
+    Definition populate_shirts_from_outfits : command :=
+      <{ for "row" in <[ "row" <- mut "outfits";
+                         ret ({"name" : "row" ["shirt_name"],
+                                 "color" : "row" ["shirt_color"],
+                                   "price" : "row" ["shirt_price"]}) ]>:
+                         set "shirts" := "row" :: mut "shirts" end }>.
+
+    Definition filter_shirts color : expr :=
+      ESort LikeList <[ "row" <- mut "shirts" ;
+                        check("row"["color"] == << EAtom (AString color) >>);
+                        ret "row" ]>.
+
+    Definition query3_1 :=
+      CLetMut (EAtom (AString ""))  "white_shirt_info"
+        (CForeach (filter_shirts "white") "r"
+          <{ let "n" = "r"["name"] +++ << EAtom (AString ": ") >> in
+            let "p" = << EUnop OIntToString (EAccess (EVar "r") "price") >> +++ << EAtom (AString "\n") >> in
+            let "line" = "n" +++ "p" in
+            set "white_shirt_info" := mut "white_shirt_info" +++ "line" }>).
+
+    Definition query3_2 :=
+      CAssign "total_shirt_price" (EFold (<["row" <- mut "shirts" ; ret "row"["price"]]>) (EAtom (AInt 0)) "v" "acc" (EBinop OPlus (EVar "v") (EVar "acc"))).
+
+    Definition query3_3 :=
+      CAssign "min_shirt_price"
+        (EFold (<["row" <- mut "shirts" ; ret "row"["price"]]>) (EAtom (ANone (Some TInt))) "v" "acc"
+           (EOptMatch (EVar "acc") (EUnop OSome (EVar "v"))
+              "x" (EIf (EBinop OLess (EVar "v") (EVar "x")) (EUnop OSome (EVar "v")) (EVar "acc")))).
+
+    Definition ex3 := CLetMut (EAtom (ANil (Some (shirts_row_ty)))) "shirts"
+                        (CSeq populate_shirts_from_outfits
+                           (CSeq query3_1
+                              (CSeq query3_2 query3_3))).
+
+    Definition init_Gstore3 : ctenv := map.put (map.put (map.put map.empty "outfits" (TList outfits_row_ty)) "total_shirt_price" TInt) "min_shirt_price" (TOption TInt).
+    Definition init_Genv3 : ctenv := map.empty.
+
+    Definition ex3_transformed := ex_transf3 init_Gstore3 init_Genv3 ex3.
+    (* Compute typecheck init_Gstore3 init_Genv3 ex3. *)
+    (* Compute ex3_transformed. *)
+
+    Theorem ex3_transformed_sem : forall (store env : clocals),
+        locals_wf init_Gstore3 store ->
+        locals_wf init_Genv3 env ->
+        interp_command store env ex3_transformed = interp_command store env ex3.
+    Proof.
+      apply transf_sound__preserve_sem; eauto using ex_transf_sound with transf_hints.
+    Qed.
+  End Example3.
+End WithConcreteMaps.
+
+Print Assumptions ex0_transformed.
+Print Assumptions ex1_transformed.
+Print Assumptions ex2_transformed.
+Print Assumptions ex3_transformed.
